Nunchaku/Frontend.lean
@@ -5,8 +5,8 @@ public import Nunchaku.Attr
 public meta import Nunchaku.Util.Model
 import Nunchaku.Transformation
 meta import Nunchaku.Transformation
-import Nunchaku.Util.NunchakuPrinter
-import Lean.Elab.Tactic.BVDecide.External
+meta import Nunchaku.Util.NunchakuPrinter
+meta import Lean.Elab.Tactic.BVDecide.External
 
 /-!
 This module contains the main entry point to the nunchaku tactic.
@@ -16,7 +16,7 @@ namespace Nunchaku
 
 open Lean Elab Tactic
 
-def runSolver (problem : NunProblem) (cfg : NunchakuConfig) :
+meta def runSolver (problem : NunProblem) (cfg : NunchakuConfig) :
     MetaM NunResult := do
   IO.FS.withTempFile fun nunHandle nunPath => do
     withTraceNode `nunchaku.solver (fun _ => return "Serializing Nunchaku Problem") do
@@ -60,7 +60,7 @@ def runSolver (problem : NunProblem) (cfg : NunchakuConfig) :
         else
           throwError s!"The external prover produced unexpected output, stdout:\n{stdout}stderr:\n{stderr}"
 
-public def runNunchaku (g : MVarId) (cfg : NunchakuConfig) : MetaM LeanResult := do
+public meta def runNunchaku (g : MVarId) (cfg : NunchakuConfig) : MetaM LeanResult := do
   TransforM.run g cfg do
     withoutModifyingEnv do
       let (problem, back) ←
